lib/coq/MachineWordTest.v
@@ -1,0 +1,209 @@
+From Sail Require Import MachineWord.
+From stdpp Require Import bitvector.
+Require Import ZArith.
+
+Import MachineWord.
+Open Scope Z.
+
+Transparent Z_to_bv
+       bv_0 bv_succ bv_pred
+       bv_add bv_sub bv_opp
+       bv_mul bv_divu bv_modu
+       bv_divs bv_quots bv_mods bv_rems
+       bv_shiftl bv_shiftr bv_ashiftr bv_or
+       bv_and bv_xor bv_not bv_zero_extend
+       bv_sign_extend bv_extract bv_concat
+       bv_add_Z bv_sub_Z bv_mul_Z
+       bool_to_bv bv_to_bits.
+
+
+Example zeros_3 : word_to_Z (zeros 3) = 0.
+reflexivity.
+Qed.
+
+Example ones_3 : word_to_Z (ones 3) = -1.
+compute.
+reflexivity.
+Qed.
+
+Example ones_3_N : word_to_N (ones 3) = 7%N.
+reflexivity.
+Qed.
+
+Example get_bit_5 :
+  get_bit (N_to_word 4 5) 0 = true /\
+  get_bit (N_to_word 4 5) 1 = false /\
+  get_bit (N_to_word 4 5) 2 = true.
+compute.
+auto.
+Qed.
+
+Example set_bit_5 :
+  set_bit (N_to_word 4 5) 0 false = N_to_word 4 4 /\
+  set_bit (N_to_word 4 5) 1 true  = N_to_word 4 7 /\
+  set_bit (N_to_word 4 5) 2 false = N_to_word 4 1 /\
+  set_bit (N_to_word 4 5) 0 true  = N_to_word 4 5 /\
+  set_bit (N_to_word 4 5) 1 false = N_to_word 4 5 /\
+  set_bit (N_to_word 4 5) 2 true  = N_to_word 4 5.
+compute.
+auto 7.
+Qed.
+
+Example word_to_bools_5 : word_to_bools (N_to_word 4 5) = [false; true; false; true].
+compute.
+reflexivity.
+Qed.
+
+Example bools_to_word_5 : N_to_word 4 5 = bools_to_word [false; true; false; true].
+reflexivity.
+Qed.
+
+Example Z_word_Z :
+  word_to_Z (Z_to_word 4 3) = 3 /\
+  word_to_Z (Z_to_word 4 5) = 5 /\
+  word_to_Z (Z_to_word 5 5) = 5 /\
+  word_to_Z (Z_to_word 10 17) = 17 /\
+  word_to_Z (Z_to_word 4 (-3)) = -3 /\
+  word_to_Z (Z_to_word 4 (-5)) = -5 /\
+  word_to_Z (Z_to_word 5 (-5)) = -5 /\
+  word_to_Z (Z_to_word 10 (-17)) = -17.
+compute.
+auto 10.
+Qed.
+
+Local Open Scope N.
+Example N_word_N :
+  word_to_N (N_to_word 4 3) = 3 /\
+  word_to_N (N_to_word 4 5) = 5 /\
+  word_to_N (N_to_word 5 5) = 5 /\
+  word_to_N (N_to_word 10 17) = 17 /\
+  word_to_N (N_to_word 4 11) = 11 /\
+  word_to_N (N_to_word 4 13) = 13 /\
+  word_to_N (N_to_word 5 21) = 21.
+compute.
+auto 10.
+Qed.
+Close Scope N.
+
+Example slice_5 : slice 2 (Z_to_word 10 5) 1 = Z_to_word 2 2.
+reflexivity.
+Qed.
+
+Example update_slice_5 : update_slice (Z_to_word 10 5) 1 (Z_to_word 2 3) = Z_to_word 10 7.
+compute.
+reflexivity.
+Qed.
+
+Example zero_extend_5 :
+  zero_extend 10 (Z_to_word 4 5) = Z_to_word 10 5 /\
+  zero_extend 10 (Z_to_word 3 5) = Z_to_word 10 5.
+compute.
+auto.
+Qed.
+
+Example sign_extend_5 :
+  sign_extend 10 (Z_to_word 4 5) = Z_to_word 10 5 /\
+  sign_extend 10 (Z_to_word 3 5) = Z_to_word 10 (-3).
+compute.
+auto.
+Qed.
+
+Example concat_5 : concat (Z_to_word 4 5) (Z_to_word 5 5) = bools_to_word [false; true; false; true; false; false; true; false; true].
+compute.
+reflexivity.
+Qed.
+
+Example and_5 :
+  eqb (and (Z_to_word 4 5) (Z_to_word 4 5)) (Z_to_word 4 5) = true /\
+  eqb (and (Z_to_word 4 7) (Z_to_word 4 5)) (Z_to_word 4 5) = true /\
+  eqb (and (Z_to_word 4 5) (Z_to_word 4 1)) (Z_to_word 4 1) = true.
+compute.
+auto.
+Qed.
+
+Example or_5 :
+  eqb (or (Z_to_word 4 5) (Z_to_word 4 5)) (Z_to_word 4 5) = true /\
+  eqb (or (Z_to_word 4 7) (Z_to_word 4 5)) (Z_to_word 4 7) = true /\
+  eqb (or (Z_to_word 4 5) (Z_to_word 4 1)) (Z_to_word 4 5) = true.
+compute.
+auto.
+Qed.
+
+Example xor_5 :
+  eqb (xor (Z_to_word 4 5) (Z_to_word 4 5)) (Z_to_word 4 0) = true /\
+  eqb (xor (Z_to_word 4 7) (Z_to_word 4 5)) (Z_to_word 4 2) = true /\
+  eqb (xor (Z_to_word 4 5) (Z_to_word 4 1)) (Z_to_word 4 4) = true.
+compute.
+auto.
+Qed.
+
+Example not_5 : eqb (not (Z_to_word 4 5)) (Z_to_word 4 (-6)) = true.
+compute.
+reflexivity.
+Qed.
+
+Example add_5 :
+  eqb (add (Z_to_word 4 5) (Z_to_word 4 0)) (Z_to_word 4 5) = true /\
+  eqb (add (Z_to_word 4 5) (Z_to_word 4 2)) (Z_to_word 4 7) = true /\
+  eqb (add (Z_to_word 4 5) (Z_to_word 4 3)) (Z_to_word 4 (-8)) = true.
+compute.
+auto.
+Qed.
+
+Example sub_5 :
+  eqb (sub (Z_to_word 4 5) (Z_to_word 4 0)) (Z_to_word 4 5) = true /\
+  eqb (sub (Z_to_word 4 5) (Z_to_word 4 2)) (Z_to_word 4 3) = true /\
+  eqb (sub (Z_to_word 4 5) (Z_to_word 4 3)) (Z_to_word 4 2) = true.
+compute.
+auto.
+Qed.
+
+Example mul_5 :
+  eqb (mul (Z_to_word 4 5) (Z_to_word 4 0)) (Z_to_word 4 0) = true /\
+  eqb (mul (Z_to_word 4 5) (Z_to_word 4 2)) (Z_to_word 4 10) = true /\
+  eqb (mul (Z_to_word 4 5) (Z_to_word 4 3)) (Z_to_word 4 15) = true.
+compute.
+auto.
+Qed.
+
+Example lsl :
+  eqb (logical_shift_left (Z_to_word 4 5) 0) (Z_to_word 4 5) = true /\
+  eqb (logical_shift_left (Z_to_word 4 5) 1) (Z_to_word 4 10) = true /\
+  eqb (logical_shift_left (Z_to_word 4 5) 3) (Z_to_word 4 8) = true.
+compute.
+auto.
+Qed.
+
+Example lsr :
+  eqb (logical_shift_right (Z_to_word 4 5) 0) (Z_to_word 4 5) = true /\
+  eqb (logical_shift_right (Z_to_word 4 5) 1) (Z_to_word 4 2) = true /\
+  eqb (logical_shift_right (Z_to_word 4 5) 3) (Z_to_word 4 0) = true.
+compute.
+auto.
+Qed.
+
+Example asr :
+  eqb (arith_shift_right (Z_to_word 4 5) 0) (Z_to_word 4 5) = true /\
+  eqb (arith_shift_right (Z_to_word 4 5) 1) (Z_to_word 4 2) = true /\
+  eqb (arith_shift_right (Z_to_word 4 5) 3) (Z_to_word 4 0) = true /\
+  eqb (arith_shift_right (Z_to_word 3 5) 0) (Z_to_word 3 5) = true /\
+  eqb (arith_shift_right (Z_to_word 3 5) 1) (Z_to_word 3 6) = true /\
+  eqb (arith_shift_right (Z_to_word 3 5) 3) (Z_to_word 3 7) = true.
+compute.
+auto 10.
+Qed.
+
+Example replicate_5 :
+  eqb (replicate 1 (Z_to_word 4 5)) (Z_to_word 4 5) = true /\
+  eqb (replicate 2 (Z_to_word 4 5)) (Z_to_word 8 85) = true /\
+  eqb (replicate 3 (Z_to_word 4 5)) (Z_to_word 12 1365) = true.
+compute.
+auto 10.
+Qed.
+
+Example reverse_endian_5 :
+  eqb (reverse_endian (Z_to_word 8 5)) (Z_to_word 8 5) = true /\
+  eqb (reverse_endian (Z_to_word 16 5)) (Z_to_word 16 1280) = true.
+compute.
+auto.
+Qed.
